ASC_Hoare.thy
@@ -113,7 +113,7 @@ next
         
   
   have rmN_calc[simp] : "{xs' \<in> cN.
-        \<not> io_reduction_on M1 M2 {xs'} \<or>
+        \<not> io_reduction_on M1 {xs'} M2 \<or>
         (\<forall>io\<in>language_state_in M1 (initial M1) {xs'}.
             \<exists>V''\<in>N io M1 V.
                \<exists>S1 vs xs.
@@ -130,7 +130,7 @@ next
 
 
     have "{xs' \<in> cN.
-          \<not> io_reduction_on M1 M2 {xs'} \<or>
+          \<not> io_reduction_on M1 {xs'} M2 \<or>
           (\<forall>io\<in>language_state_in M1 (initial M1) {xs'}.
               \<exists>V''\<in>N io M1 V.
                  \<exists>S1 vs xs.
@@ -143,7 +143,7 @@ next
                            (\<forall>io1\<in>RP M2 s1 vs xs V''. \<forall>io2\<in>RP M2 s2 vs xs V''. B M1 io1 \<Omega> \<noteq> B M1 io2 \<Omega>)) \<and>
                     m < LB M2 M1 vs xs (tsN \<union> V) S1 \<Omega> V'')} =
           {xs' \<in> C M2 M1 \<Omega> V m (Suc k).
-          \<not> io_reduction_on M1 M2 {xs'} \<or>
+          \<not> io_reduction_on M1 {xs'} M2 \<or>
           (\<forall>io\<in>language_state_in M1 (initial M1) {xs'}.
               \<exists>V''\<in>N io M1 V.
                  \<exists>S1 vs xs.
@@ -158,7 +158,7 @@ next
       using \<open>cN = C M2 M1 \<Omega> V m (Suc k)\<close> \<open>tsN = TS M2 M1 \<Omega> V m k\<close> by blast
     
     moreover have "{xs' \<in> C M2 M1 \<Omega> V m (Suc k).
-                    \<not> io_reduction_on M1 M2 {xs'} \<or>
+                    \<not> io_reduction_on M1 {xs'} M2 \<or>
                     (\<forall>io\<in>language_state_in M1 (initial M1) {xs'}.
                         \<exists>V''\<in>N io M1 V.
                            \<exists>S1 vs xs.
@@ -173,7 +173,7 @@ next
                     RM M2 M1 \<Omega> V m (Suc k)"
       using RM.simps(2)[of M2 M1 \<Omega> V m k] by blast
     ultimately have "{xs' \<in> cN.
-                      \<not> io_reduction_on M1 M2 {xs'} \<or>
+                      \<not> io_reduction_on M1 {xs'} M2 \<or>
                       (\<forall>io\<in>language_state_in M1 (initial M1) {xs'}.
                           \<exists>V''\<in>N io M1 V.
                              \<exists>S1 vs xs.
@@ -192,7 +192,7 @@ next
   qed
   moreover have "RM M2 M1 \<Omega> V m iter = RM M2 M1 \<Omega> V m (iter + 1 - 1)" by simp
   ultimately have rmN_calc' : "{xs' \<in> cN.
-        \<not> io_reduction_on M1 M2 {xs'} \<or>
+        \<not> io_reduction_on M1 {xs'} M2 \<or>
         (\<forall>io\<in>language_state_in M1 (initial M1) {xs'}.
             \<exists>V''\<in>N io M1 V.
                \<exists>S1 vs xs.
@@ -227,7 +227,7 @@ next
   have cN_calc : "append_set
         (cN -
          {xs' \<in> cN.
-          \<not> io_reduction_on M1 M2 {xs'} \<or>
+          \<not> io_reduction_on M1 {xs'} M2 \<or>
           (\<forall>io\<in>language_state_in M1 (initial M1) {xs'}.
               \<exists>V''\<in>N io M1 V.
                  \<exists>S1 vs xs.
@@ -247,7 +247,7 @@ next
     have "append_set
           (cN -
            {xs' \<in> cN.
-            \<not> io_reduction_on M1 M2 {xs'} \<or>
+            \<not> io_reduction_on M1 {xs'} M2 \<or>
             (\<forall>io\<in>language_state_in M1 (initial M1) {xs'}.
                 \<exists>V''\<in>N io M1 V.
                    \<exists>S1 vs xs.
@@ -296,7 +296,7 @@ next
               (append_set
                 (cN -
                  {xs' \<in> cN.
-                  \<not> io_reduction_on M1 M2 {xs'} \<or>
+                  \<not> io_reduction_on M1 {xs'} M2 \<or>
                   (\<forall>io\<in>language_state_in M1 (initial M1) {xs'}.
                       \<exists>V''\<in>N io M1 V.
                          \<exists>S1 vs xs.
@@ -317,7 +317,7 @@ next
                (append_set
                  (cN -
                   {xs' \<in> cN.
-                   \<not> io_reduction_on M1 M2 {xs'} \<or>
+                   \<not> io_reduction_on M1 {xs'} M2 \<or>
                    (\<forall>io\<in>language_state_in M1 (initial M1) {xs'}.
                        \<exists>V''\<in>N io M1 V.
                           \<exists>S1 vs xs.
@@ -339,7 +339,7 @@ next
               (append_set
                 (cN -
                  {xs' \<in> cN.
-                  \<not> io_reduction_on M1 M2 {xs'} \<or>
+                  \<not> io_reduction_on M1 {xs'} M2 \<or>
                   (\<forall>io\<in>language_state_in M1 (initial M1) {xs'}.
                       \<exists>V''\<in>N io M1 V.
                          \<exists>S1 vs xs.
@@ -360,7 +360,7 @@ next
                       (append_set
                         (cN -
                          {xs' \<in> cN.
-                          \<not> io_reduction_on M1 M2 {xs'} \<or>
+                          \<not> io_reduction_on M1 {xs'} M2 \<or>
                           (\<forall>io\<in>language_state_in M1 (initial M1) {xs'}.
                               \<exists>V''\<in>N io M1 V.
                                  \<exists>S1 vs xs.
@@ -384,7 +384,7 @@ next
                       (append_set
                         (cN -
                          {xs' \<in> cN.
-                          \<not> io_reduction_on M1 M2 {xs'} \<or>
+                          \<not> io_reduction_on M1 {xs'} M2 \<or>
                           (\<forall>io\<in>language_state_in M1 (initial M1) {xs'}.
                               \<exists>V''\<in>N io M1 V.
                                  \<exists>S1 vs xs.
@@ -405,7 +405,7 @@ next
                                (append_set
                                  (cN -
                                   {xs' \<in> cN.
-                                   \<not> io_reduction_on M1 M2 {xs'} \<or>
+                                   \<not> io_reduction_on M1 {xs'} M2 \<or>
                                    (\<forall>io\<in>language_state_in M1 (initial M1) {xs'}.
                                        \<exists>V''\<in>N io M1 V.
                                           \<exists>S1 vs xs.
@@ -432,7 +432,7 @@ next
               (append_set
                 (cN -
                  {xs' \<in> cN.
-                  \<not> io_reduction_on M1 M2 {xs'} \<or>
+                  \<not> io_reduction_on M1 {xs'} M2 \<or>
                   (\<forall>io\<in>language_state_in M1 (initial M1) {xs'}.
                       \<exists>V''\<in>N io M1 V.
                          \<exists>S1 vs xs.
@@ -453,7 +453,7 @@ next
                (append_set
                  (cN -
                   {xs' \<in> cN.
-                   \<not> io_reduction_on M1 M2 {xs'} \<or>
+                   \<not> io_reduction_on M1 {xs'} M2 \<or>
                    (\<forall>io\<in>language_state_in M1 (initial M1) {xs'}.
                        \<exists>V''\<in>N io M1 V.
                           \<exists>S1 vs xs.
@@ -475,7 +475,7 @@ next
               (append_set
                 (cN -
                  {xs' \<in> cN.
-                  \<not> io_reduction_on M1 M2 {xs'} \<or>
+                  \<not> io_reduction_on M1 {xs'} M2 \<or>
                   (\<forall>io\<in>language_state_in M1 (initial M1) {xs'}.
                       \<exists>V''\<in>N io M1 V.
                          \<exists>S1 vs xs.
@@ -496,7 +496,7 @@ next
                       (append_set
                         (cN -
                          {xs' \<in> cN.
-                          \<not> io_reduction_on M1 M2 {xs'} \<or>
+                          \<not> io_reduction_on M1 {xs'} M2 \<or>
                           (\<forall>io\<in>language_state_in M1 (initial M1) {xs'}.
                               \<exists>V''\<in>N io M1 V.
                                  \<exists>S1 vs xs.
@@ -520,7 +520,7 @@ next
                       (append_set
                         (cN -
                          {xs' \<in> cN.
-                          \<not> io_reduction_on M1 M2 {xs'} \<or>
+                          \<not> io_reduction_on M1 {xs'} M2 \<or>
                           (\<forall>io\<in>language_state_in M1 (initial M1) {xs'}.
                               \<exists>V''\<in>N io M1 V.
                                  \<exists>S1 vs xs.
@@ -541,7 +541,7 @@ next
                                (append_set
                                  (cN -
                                   {xs' \<in> cN.
-                                   \<not> io_reduction_on M1 M2 {xs'} \<or>
+                                   \<not> io_reduction_on M1 {xs'} M2 \<or>
                                    (\<forall>io\<in>language_state_in M1 (initial M1) {xs'}.
                                        \<exists>V''\<in>N io M1 V.
                                           \<exists>S1 vs xs.
@@ -588,7 +588,7 @@ next
        append_set
         (cN -
          {xs' \<in> cN.
-          \<not> io_reduction_on M1 M2 {xs'} \<or>
+          \<not> io_reduction_on M1 {xs'} M2 \<or>
           (\<forall>io\<in>language_state_in M1 (initial M1) {xs'}.
               \<exists>V''\<in>N io M1 V.
                  \<exists>S1 vs xs.
@@ -605,7 +605,7 @@ next
        (tsN \<union> cN) =
        C M2 M1 \<Omega> V m (iter + 1) \<and>
        {xs' \<in> cN.
-        \<not> io_reduction_on M1 M2 {xs'} \<or>
+        \<not> io_reduction_on M1 {xs'} M2 \<or>
         (\<forall>io\<in>language_state_in M1 (initial M1) {xs'}.
             \<exists>V''\<in>N io M1 V.
                \<exists>S1 vs xs.
@@ -623,7 +623,7 @@ next
               (append_set
                 (cN -
                  {xs' \<in> cN.
-                  \<not> io_reduction_on M1 M2 {xs'} \<or>
+                  \<not> io_reduction_on M1 {xs'} M2 \<or>
                   (\<forall>io\<in>language_state_in M1 (initial M1) {xs'}.
                       \<exists>V''\<in>N io M1 V.
                          \<exists>S1 vs xs.
@@ -644,7 +644,7 @@ next
                (append_set
                  (cN -
                   {xs' \<in> cN.
-                   \<not> io_reduction_on M1 M2 {xs'} \<or>
+                   \<not> io_reduction_on M1 {xs'} M2 \<or>
                    (\<forall>io\<in>language_state_in M1 (initial M1) {xs'}.
                        \<exists>V''\<in>N io M1 V.
                           \<exists>S1 vs xs.
@@ -665,7 +665,7 @@ next
               (append_set
                 (cN -
                  {xs' \<in> cN.
-                  \<not> io_reduction_on M1 M2 {xs'} \<or>
+                  \<not> io_reduction_on M1 {xs'} M2 \<or>
                   (\<forall>io\<in>language_state_in M1 (initial M1) {xs'}.
                       \<exists>V''\<in>N io M1 V.
                          \<exists>S1 vs xs.
@@ -686,7 +686,7 @@ next
                (append_set
                  (cN -
                   {xs' \<in> cN.
-                   \<not> io_reduction_on M1 M2 {xs'} \<or>
+                   \<not> io_reduction_on M1 {xs'} M2 \<or>
                    (\<forall>io\<in>language_state_in M1 (initial M1) {xs'}.
                        \<exists>V''\<in>N io M1 V.
                           \<exists>S1 vs xs.
